---
tags: [2nde/06-Racines-Carrees/Exos]
title: 2nde-Chap-06-Racines-Carrees-Exos
created: '2022-08-10T19:52:45.897Z'
modified: '2022-08-23T10:54:11.504Z'
---

# 2nde-Chap-06-Racines-Carrees-Exos

Tags : 2nde/06-Racines-Carrees/Exos


### Exercice II :
Simplifier :

1.  $A=2\sqrt{3} - \sqrt{300} + 3\sqrt{12}$


2.  $B=\sqrt{40} + \sqrt{90} - \sqrt{490}$

3.  $C=\sqrt{18} + \sqrt{50} - \sqrt{32} + \sqrt{200}$

4.  $D=\sqrt{250} - \sqrt{490} - 2\sqrt{81}$

5.  $E=\sqrt{2} + 3\sqrt{8} - 6\sqrt{50}$

6.  $F=- 4\sqrt{24} - \sqrt{6} + 4\sqrt{54} + 3\sqrt{24}$

7.  $G=3\sqrt{2}(\sqrt{2} + 1)$

8.  $H=(2\sqrt{5} + 2)(1 - 3\sqrt{5})$

9.  $I=(5\sqrt{2} - 4)(3 - 8\sqrt{2})$

10.  $J=(3\sqrt{2} - \sqrt{3})(\sqrt{2} + \sqrt{3})$

11. $K=4\sqrt{54} - 4\sqrt{6} + 2\sqrt{24} + 2\sqrt{24}$

12. $L=\sqrt{2}(\sqrt{2} - 1) + \sqrt{3}(\sqrt{3} - \sqrt{6})$

13. $M=2\sqrt{7}(1 - 3\sqrt{7})(2\sqrt{7} - 3)$

14. $N={(\sqrt{2}(1 + \sqrt{3}))}^{2}$

15. $O={(2 - \sqrt{3})}^{2}$

16. $P={(\sqrt{2} - \sqrt{5})}^{2}$

17. $Q={(\sqrt{6} - \sqrt{8})}^{2}$

18. $R=\dfrac{(\sqrt{45} + 5)(\sqrt{5} - 3)}{4}$

19. $S=\sqrt{5} \times \frac{(\sqrt{19} - \sqrt{13})(\sqrt{19} + \sqrt{13})}{6}$

20. $T=4\sqrt{3} + 2\sqrt{48}$

21. $U=- 2\sqrt{8} + 3\sqrt{50} - 7\sqrt{18}$

22. $V=3\sqrt{15} \times 2\sqrt{35} - 2\sqrt{84} - 7\dfrac{\sqrt{105}}{\sqrt{5}}$

23. $W=\frac{\sqrt{7}}{\sqrt{6}} \times (\dfrac{\sqrt{14 \times 15}}{\sqrt{5}})$

24. $X=\dfrac{\sqrt{12^{2}} + \sqrt{9^{2}}}{\sqrt{(12^{2} + 9^{2})}}$

25. $Y=2\sqrt{21}\dfrac{\sqrt{75}}{\sqrt{35}\sqrt{20}}$

26. $Z=\sqrt{176} \times (\dfrac{\sqrt{99}}{\sqrt{49}})$
---
### Exercice III :
Écrire sans racines au dénominateur :

1.  $A=\sqrt{2} + \sqrt{\frac{1}{2}} - \sqrt{\frac{1}{8}}$

2.  $B=\dfrac{\sqrt{3}}{\sqrt{3} - 2}$

3.  $C=\dfrac{1}{\sqrt{5} - \sqrt{3}}$

4. $D= \sqrt{\dfrac{30}{7}} \times \sqrt{\dfrac{21}{40}}$

5.  $E=\dfrac{1}{\sqrt{5} + \sqrt{3}}$

6.  $F=\dfrac{1 + \sqrt{3}}{2 - \sqrt{3}}$

7.  $G=\dfrac{\sqrt{3} + 3}{\sqrt{3} - 3}$

8.  $H=\dfrac{\sqrt{7} + \sqrt{5}}{\sqrt{7} - \sqrt{5}}$

9.  $I=\dfrac{\sqrt{7} - \sqrt{5}}{\sqrt{7} + \sqrt{5}}$

10.  $J=\dfrac{\sqrt{10} + \sqrt{5}}{\sqrt{10} - \sqrt{5}}$

11. $K=\dfrac{\sqrt{7}}{\sqrt{2} - \sqrt{7}}$

12. $L=\dfrac{4}{1 + \sqrt{3}}$

13. $M=(\sqrt{3} - \sqrt{27} + \sqrt{12})\dfrac{\sqrt{3}}{\sqrt{54}}$

14. $N=\dfrac{3}{\sqrt{5} - 2}$

15. $O=2 \times \dfrac{\sqrt{5}}{1 - \sqrt{45}}$

16. $P=\dfrac{\sqrt{63} - 5\sqrt{7}}{\sqrt{28}}$

17. $Q=\dfrac{\sqrt{243} - \sqrt{147}}{\sqrt{12}}$

18. $R=\dfrac{\sqrt{3} + \sqrt{2}}{\sqrt{3} - \sqrt{2}} + \dfrac{\sqrt{3} - \sqrt{2}}{\sqrt{3} + \sqrt{2}}$

19. $S=\dfrac{\sqrt{{( - 7)}^{2}}}{4\sqrt{2} - \sqrt{8}}$
---
### Exercice IV : 
Simplifier :

1.  $A=\dfrac{2\sqrt{21}\sqrt{75a^{2}}}{\sqrt{35}\sqrt{20}}$


2.  $B= {(\dfrac{\sqrt{10 - 2\sqrt{5}}}{4})}^{2} + {(\dfrac{1 + \sqrt{5}}{4})}^{2}$

3.  $C= (\sqrt{2} - \sqrt{3})(5\sqrt{2} - \sqrt{3}) - {(3\sqrt{6} + 1)}^{2}$

4.  $D= {(\sqrt{2} + \sqrt{7})}^{3}$

5.  $E= {(\sqrt{\dfrac{5}{3}} - \sqrt{\dfrac{3}{5}})}^{2}$

6.  $F= \dfrac{{(\sqrt{3} - 2)}^{2}}{\sqrt{7}} \times \dfrac{7 + 4\sqrt{3}}{\sqrt{14}}$

7.  $G= {(\sqrt{5})}^{3}{(\sqrt{5})}^{3}{(\sqrt{2})}^{3}$

8.  $H= {(2a + \sqrt{b})}^{2} + {(1 - 2a\sqrt{b})}^{2} - {(2a\sqrt{b})}^{2}$

9.  $I=\dfrac{\sqrt{3}}{\sqrt{3}–\dfrac{2}{\sqrt{3}–\dfrac{2}{\sqrt{3}}}}$

10.  $J= \dfrac{3\sqrt{5} + \sqrt{20}}{\sqrt{45}\left( 2 - \dfrac{5}{6} + \dfrac{4}{3} \right)(1 - \sqrt{3})}$

11. $K={(4 + 3\sqrt{2})}^{2} - (2 + \sqrt{2})(\sqrt{2} - 1)$

12. $L= \sqrt{\dfrac{7 + 4\sqrt{3}}{7 - 4\sqrt{3}}} + \sqrt{\dfrac{7 - 4\sqrt{3}}{7 + 4\sqrt{3}}}$

13. $M=\dfrac{\sqrt{0,04}}{\sqrt{0,0016}} + \dfrac{\sqrt{0,01}}{\sqrt{0,04}}$

14. $N={(\sqrt{2 - \sqrt{2}} + \sqrt{2 + \sqrt{2}})}^{2}$

15. $O=\sqrt{\dfrac{a^{6} + a^{6} + a^{6} + a^{6}}{5^{2} + 5^{2} + 5^{2} + 5^{2}}}$

16. $P=\sqrt{6 - \sqrt{6 - \sqrt{6 - \sqrt{6 - \sqrt{\dfrac{4\sqrt{27}}{3\sqrt{3}}}}}}}$

17. $Q=\sqrt{\dfrac{48a^{6}b^{12}}{243{(\text{ab})}^{4}}}$

18. $R=\sqrt{\dfrac{4^{80} + 5 \times 8^{53}}{28 \times 2^{155}}}$

19. $S={(\sqrt{1 + \sqrt{1 - a^{2}}} + \sqrt{1 - \sqrt{1 - a^{2}}})}^{2}$    $(a ∈ [0 ; 1])$



