---
tags: [2nde/03-Equations/Exos]
title: 2nde-Chap-03-Equations-Exos
created: '2022-08-10T19:52:45.746Z'
modified: '2022-08-11T13:48:23.573Z'
---

# 2nde-Chap-03-Equations-Exos

Tag : 2nde/03-Equations/Exos

# Chap-03-Exercices-Fiche-2-Ã‰quations

**1)**  $(0,1x - 1)(0,2x - 2)(0,03x - 0,3) = 0$


**2)**  $\dfrac{2x + 3}{5x - 1} = 2$

**3)**  $\dfrac{3}{x} = \dfrac{x}{5}$

**4)**  $x^{4} - 1 = 0$

**5)** $(x - 2)(x + 1) - x = - 2$

**6)**  $16x^{2} - 8x + 1 = 0$

**7)** $\dfrac{x^{2} + 1}{x - 1} = \dfrac{2x}{x - 1}$

**8)**  ${(x - 2)}^{2} = \dfrac{1}{16}{(5 - 2x)}^{2}$

**9)**  $\dfrac{x - \dfrac{4}{x}}{x - 2} = \dfrac{x + 2}{x}$

**10)**  $4\sqrt{7}x - 0,8 = 2\sqrt{7} - 1,6x$

**11)** $(x + 1)(3 - 2x) = 4x^{2} - 9$

**12)** $\dfrac{x^{2}}{1 - 2x} = - 1$

**13)** ${(x + 2)}^{2} = 2(x^{2} - 4)$

**14)** $\dfrac{x^{2} + x + 1}{2x - 3} = \dfrac{1}{2}$

**15)** $\dfrac{1}{x(x + 1)} = \dfrac{1}{x} - \dfrac{1}{x + 1}$

**16)** $(x + 3)(x - 7) - (x - 1)(x + 2) = 0$

**17)** $\dfrac{(x^{2} - 2x + 1)(x + 1)}{(x - 1)(x^{2} - 1)} = 1$

**18)** $x^{3} - x = 2x^{2} - 2$

**19)** $\dfrac{1}{x + 2} = \dfrac{1}{x^{2} - 4}$

**20)** ${(2x - 6)}^{2} + x - 3 = 0$

**21)** $\dfrac{2x - 2}{x - 1} = 2x$

**22)** $9x^{2} + \dfrac{1}{9} = 2x$

**23)** $\dfrac{1}{x} + \dfrac{1}{x + 1} = 2$

**24)** $(x^{2} - 9)(2x + 1) = (x + 3){(2x + 1)}^{2}$

**25)** $\dfrac{2}{x - 1} = 1 - \dfrac{x}{x + 1}$

**26)** ${(2x + 5)}^{2} - 2(7x + 4) = 4{(x + 3)}^{2} - 1$

**27)** ${(3x + 2)}^{2} = {(x - 5)}^{2}$

**28)** $2x - 3 = \dfrac{9(2x - 3)}{x^{2} - 4x + 4}$

**29)** $\dfrac{x^{2} - 1}{{(x - 1)}^{2}} = \dfrac{1}{x - 1}$

**30)** $x^{2} - x - \dfrac{3x}{x + 1} = 0$

**31)** ${(\pi - 4x)}^{2} - \pi^{2} = - 8x(\pi - 2x)$

**32)** $\dfrac{1}{x + 1} = \dfrac{1}{1 - x}$

**33)** $\dfrac{x^{2}}{16} + \dfrac{x}{2} + 1 = 0$

**34)** $\dfrac{5}{x + 3} + 1 = \dfrac{x - 1}{x + 2}$

**35)** $\dfrac{x^{2} - 2}{x^{2} - 1} = 0$

**36)** $\dfrac{9x^{2} - 4}{{(3x + 2)}^{2}} = 0$

**37)** $\dfrac{x^{2} + 2x + 1}{x^{2} - 1} = 0$

**38)** $\dfrac{x^{3} - 2x^{2} + x}{x} = 0$

**39)** ${(2x + 1)}^{2} - 3(x + \dfrac{1}{2}) = 0$

**40)** $\dfrac{1}{(x + 1)(x + 2)} + \dfrac{1}{(x + 2)(x + 3)} = 0$

**41)** $4 = {(x\sqrt{2} - 1)}^{2}$

**42)** ${(2x - 4)}^{2} + (5x - 20)(2 - x) = 0$

**43)** ${(1 - 3x)}^{2} - 5 = 0$

**44)** $\dfrac{{(4x^{2} - 25)}^{2}}{{(2x + 5)}^{2}} = 1$

**45)** $\dfrac{(x^{2} - 4)(x + 1)}{x + 2} = \dfrac{(2 - x)(x^{2} - 1)}{x - 1}$

**46)** $\dfrac{x + 1}{x} = \dfrac{x - 2}{x + 1}$

**47)** $\dfrac{2x - 3}{x + 1} = \dfrac{2x + 3}{x - 2}$

**48)** $\dfrac{2x}{x + 1} = \dfrac{x + 1}{8x}$

**49)** $5x^{4} = 10x^{3} - 5x^{2}$

**50)** $\dfrac{x^{2} + 1}{x^{2} - 4} = \dfrac{3}{x + 2} - \dfrac{3}{x - 2}$
